Test/dafny0/Datatypes.bpl
@@ -1,0 +1,306 @@
+// Dafny program verifier version 2.00, Copyright (c) 2003-2009, Microsoft.
+// Command Line Options: Datatypes.dfy /dprint:- /print:Datatyps.bpl
+
+type ref;
+
+const null: ref;
+
+type Set T = [T]bool;
+
+function Set#Empty<T>() returns (Set T);
+
+axiom (forall<T> o: T :: { Set#Empty()[o] } !Set#Empty()[o]);
+
+function Set#Singleton<T>(T) returns (Set T);
+
+axiom (forall<T> r: T :: { Set#Singleton(r) } Set#Singleton(r)[r]);
+
+axiom (forall<T> r: T, o: T :: { Set#Singleton(r)[o] } Set#Singleton(r)[o] <==> r == o);
+
+function Set#UnionOne<T>(Set T, T) returns (Set T);
+
+axiom (forall<T> a: Set T, x: T, o: T :: { Set#UnionOne(a, x)[o] } Set#UnionOne(a, x)[o] <==> o == x || a[o]);
+
+function Set#Union<T>(Set T, Set T) returns (Set T);
+
+axiom (forall<T> a: Set T, b: Set T, o: T :: { Set#Union(a, b)[o] } Set#Union(a, b)[o] <==> a[o] || b[o]);
+
+function Set#Intersection<T>(Set T, Set T) returns (Set T);
+
+axiom (forall<T> a: Set T, b: Set T, o: T :: { Set#Intersection(a, b)[o] } Set#Intersection(a, b)[o] <==> a[o] && b[o]);
+
+function Set#Difference<T>(Set T, Set T) returns (Set T);
+
+axiom (forall<T> a: Set T, b: Set T, o: T :: { Set#Difference(a, b)[o] } Set#Difference(a, b)[o] <==> a[o] && !b[o]);
+
+function Set#Subset<T>(Set T, Set T) returns (bool);
+
+axiom (forall<T> a: Set T, b: Set T :: { Set#Subset(a, b) } Set#Subset(a, b) <==> (forall o: T :: { a[o] } { b[o] } a[o] ==> b[o]));
+
+function Set#Equal<T>(Set T, Set T) returns (bool);
+
+axiom (forall<T> a: Set T, b: Set T :: { Set#Equal(a, b) } Set#Equal(a, b) <==> (forall o: T :: { a[o] } { b[o] } a[o] <==> b[o]));
+
+axiom (forall<T> a: Set T, b: Set T :: { Set#Equal(a, b) } Set#Equal(a, b) ==> a == b);
+
+function Set#Disjoint<T>(Set T, Set T) returns (bool);
+
+axiom (forall<T> a: Set T, b: Set T :: { Set#Disjoint(a, b) } Set#Disjoint(a, b) <==> (forall o: T :: { a[o] } { b[o] } !a[o] || !b[o]));
+
+type Seq _;
+
+function Seq#Length<T>(Seq T) returns (int);
+
+axiom (forall<T> s: Seq T :: { Seq#Length(s) } 0 <= Seq#Length(s));
+
+function Seq#Empty<T>() returns (Seq T);
+
+axiom (forall<T>  :: Seq#Length(Seq#Empty(): Seq T) == 0);
+
+axiom (forall<T> s: Seq T :: { Seq#Length(s) } Seq#Length(s) == 0 ==> s == Seq#Empty());
+
+function Seq#Singleton<T>(T) returns (Seq T);
+
+axiom (forall<T> t: T :: { Seq#Length(Seq#Singleton(t)) } Seq#Length(Seq#Singleton(t)) == 1);
+
+function Seq#Build<T>(s: Seq T, index: int, val: T, newLength: int) returns (Seq T);
+
+axiom (forall<T> s: Seq T, i: int, v: T, len: int :: { Seq#Length(Seq#Build(s, i, v, len)) } 0 <= len ==> Seq#Length(Seq#Build(s, i, v, len)) == len);
+
+function Seq#Append<T>(Seq T, Seq T) returns (Seq T);
+
+axiom (forall<T> s0: Seq T, s1: Seq T :: { Seq#Length(Seq#Append(s0, s1)) } Seq#Length(Seq#Append(s0, s1)) == Seq#Length(s0) + Seq#Length(s1));
+
+function Seq#Index<T>(Seq T, int) returns (T);
+
+axiom (forall<T> t: T :: { Seq#Index(Seq#Singleton(t), 0) } Seq#Index(Seq#Singleton(t), 0) == t);
+
+axiom (forall<T> s0: Seq T, s1: Seq T, n: int :: { Seq#Index(Seq#Append(s0, s1), n) } (n < Seq#Length(s0) ==> Seq#Index(Seq#Append(s0, s1), n) == Seq#Index(s0, n)) && (Seq#Length(s0) <= n ==> Seq#Index(Seq#Append(s0, s1), n) == Seq#Index(s1, n - Seq#Length(s0))));
+
+axiom (forall<T> s: Seq T, i: int, v: T, len: int, n: int :: { Seq#Index(Seq#Build(s, i, v, len), n) } 0 <= n && n < len ==> (i == n ==> Seq#Index(Seq#Build(s, i, v, len), n) == v) && (i != n ==> Seq#Index(Seq#Build(s, i, v, len), n) == Seq#Index(s, n)));
+
+function Seq#Update<T>(Seq T, int, T) returns (Seq T);
+
+axiom (forall<T> s: Seq T, i: int, v: T :: { Seq#Length(Seq#Update(s, i, v)) } 0 <= i && i < Seq#Length(s) ==> Seq#Length(Seq#Update(s, i, v)) == Seq#Length(s));
+
+axiom (forall<T> s: Seq T, i: int, v: T, n: int :: { Seq#Index(Seq#Update(s, i, v), n) } 0 <= n && n < Seq#Length(s) ==> (i == n ==> Seq#Index(Seq#Update(s, i, v), n) == v) && (i != n ==> Seq#Index(Seq#Update(s, i, v), n) == Seq#Index(s, n)));
+
+function Seq#Contains<T>(Seq T, T) returns (bool);
+
+axiom (forall<T> s: Seq T, x: T :: { Seq#Contains(s, x) } Seq#Contains(s, x) <==> (exists i: int :: { Seq#Index(s, i) } 0 <= i && i < Seq#Length(s) && Seq#Index(s, i) == x));
+
+axiom (forall x: ref :: { Seq#Contains(Seq#Empty(), x) } !Seq#Contains(Seq#Empty(), x));
+
+axiom (forall<T> s0: Seq T, s1: Seq T, x: T :: { Seq#Contains(Seq#Append(s0, s1), x) } Seq#Contains(Seq#Append(s0, s1), x) <==> Seq#Contains(s0, x) || Seq#Contains(s1, x));
+
+axiom (forall<T> s: Seq T, i: int, v: T, len: int, x: T :: { Seq#Contains(Seq#Build(s, i, v, len), x) } Seq#Contains(Seq#Build(s, i, v, len), x) <==> (0 <= i && i < len && x == v) || (exists j: int :: { Seq#Index(s, j) } 0 <= j && j < Seq#Length(s) && j < len && j != i && Seq#Index(s, j) == x));
+
+axiom (forall<T> s: Seq T, n: int, x: T :: { Seq#Contains(Seq#Take(s, n), x) } Seq#Contains(Seq#Take(s, n), x) <==> (exists i: int :: { Seq#Index(s, i) } 0 <= i && i < n && i < Seq#Length(s) && Seq#Index(s, i) == x));
+
+axiom (forall<T> s: Seq T, n: int, x: T :: { Seq#Contains(Seq#Drop(s, n), x) } Seq#Contains(Seq#Drop(s, n), x) <==> (exists i: int :: { Seq#Index(s, i) } 0 <= n && n <= i && i < Seq#Length(s) && Seq#Index(s, i) == x));
+
+function Seq#Equal<T>(Seq T, Seq T) returns (bool);
+
+axiom (forall<T> s0: Seq T, s1: Seq T :: { Seq#Equal(s0, s1) } Seq#Equal(s0, s1) <==> Seq#Length(s0) == Seq#Length(s1) && (forall j: int :: { Seq#Index(s0, j) } { Seq#Index(s1, j) } 0 <= j && j < Seq#Length(s0) ==> Seq#Index(s0, j) == Seq#Index(s1, j)));
+
+axiom (forall<T> a: Seq T, b: Seq T :: { Seq#Equal(a, b) } Seq#Equal(a, b) ==> a == b);
+
+function Seq#SameUntil<T>(Seq T, Seq T, int) returns (bool);
+
+axiom (forall<T> s0: Seq T, s1: Seq T, n: int :: { Seq#SameUntil(s0, s1, n) } Seq#SameUntil(s0, s1, n) <==> (forall j: int :: { Seq#Index(s0, j) } { Seq#Index(s1, j) } 0 <= j && j < n ==> Seq#Index(s0, j) == Seq#Index(s1, j)));
+
+function Seq#Take<T>(Seq T, howMany: int) returns (Seq T);
+
+axiom (forall<T> s: Seq T, n: int :: { Seq#Length(Seq#Take(s, n)) } 0 <= n ==> (n <= Seq#Length(s) ==> Seq#Length(Seq#Take(s, n)) == n) && (Seq#Length(s) < n ==> Seq#Length(Seq#Take(s, n)) == Seq#Length(s)));
+
+axiom (forall<T> s: Seq T, n: int, j: int :: { Seq#Index(Seq#Take(s, n), j) } 0 <= j && j < n && j < Seq#Length(s) ==> Seq#Index(Seq#Take(s, n), j) == Seq#Index(s, j));
+
+function Seq#Drop<T>(Seq T, howMany: int) returns (Seq T);
+
+axiom (forall<T> s: Seq T, n: int :: { Seq#Length(Seq#Drop(s, n)) } 0 <= n ==> (n <= Seq#Length(s) ==> Seq#Length(Seq#Drop(s, n)) == Seq#Length(s) - n) && (Seq#Length(s) < n ==> Seq#Length(Seq#Drop(s, n)) == 0));
+
+axiom (forall<T> s: Seq T, n: int, j: int :: { Seq#Index(Seq#Drop(s, n), j) } 0 <= n && 0 <= j && j < Seq#Length(s) - n ==> Seq#Index(Seq#Drop(s, n), j) == Seq#Index(s, j + n));
+
+type BoxType;
+
+function $Box<T>(T) returns (BoxType);
+
+function $Unbox<T>(BoxType) returns (T);
+
+axiom (forall<T> x: T :: { $Box(x) } $Unbox($Box(x)) == x);
+
+axiom (forall b: BoxType :: { $Unbox(b): int } $Box($Unbox(b): int) == b);
+
+axiom (forall b: BoxType :: { $Unbox(b): ref } $Box($Unbox(b): ref) == b);
+
+axiom (forall b: BoxType :: { $Unbox(b): Set BoxType } $Box($Unbox(b): Set BoxType) == b);
+
+axiom (forall b: BoxType :: { $Unbox(b): Seq BoxType } $Box($Unbox(b): Seq BoxType) == b);
+
+type ClassName;
+
+const unique class.int: ClassName;
+
+const unique class.bool: ClassName;
+
+const unique class.object: ClassName;
+
+const unique class.set: ClassName;
+
+const unique class.seq: ClassName;
+
+function dtype(ref) returns (ClassName);
+
+function TypeParams(ref, int) returns (ClassName);
+
+function TypeTuple(a: ClassName, b: ClassName) returns (ClassName);
+
+function TypeTupleCar(ClassName) returns (ClassName);
+
+function TypeTupleCdr(ClassName) returns (ClassName);
+
+axiom (forall a: ClassName, b: ClassName :: { TypeTuple(a, b) } TypeTupleCar(TypeTuple(a, b)) == a && TypeTupleCdr(TypeTuple(a, b)) == b);
+
+type DatatypeType;
+
+type Field _;
+
+type HeapType = <alpha>[ref,Field alpha]alpha;
+
+function $IsGoodHeap(HeapType) returns (bool);
+
+var $Heap: HeapType where $IsGoodHeap($Heap) && #cev_var_update(#cev_pc, cev_implicit, #loc.$Heap, $Heap);
+
+const unique #loc.$Heap: $token;
+
+const unique alloc: Field bool;
+
+function DeclType<T>(Field T) returns (ClassName);
+
+function $HeapSucc(HeapType, HeapType) returns (bool);
+
+axiom (forall h: HeapType, k: HeapType :: { $HeapSucc(h, k) } $HeapSucc(h, k) ==> (forall o: ref :: { k[o, alloc] } h[o, alloc] ==> k[o, alloc]));
+
+axiom (forall x: int, y: int :: { x % y } { x / y } x % y == x - x / y * y);
+
+axiom (forall x: int, y: int :: { x % y } 0 < y ==> 0 <= x % y && x % y < y);
+
+axiom (forall x: int, y: int :: { x % y } y < 0 ==> y < x % y && x % y <= 0);
+
+axiom (forall a: int, b: int, d: int :: { a % d, b % d } 2 <= d && a % d == b % d && a < b ==> a + d <= b);
+
+type $token;
+
+function $file_name_is(id: int, tok: $token) returns (bool);
+
+type cf_event;
+
+type var_locglob;
+
+const unique conditional_moment: cf_event;
+
+const unique took_then_branch: cf_event;
+
+const unique took_else_branch: cf_event;
+
+const unique loop_register: cf_event;
+
+const unique loop_entered: cf_event;
+
+const unique loop_exited: cf_event;
+
+const unique cev_local: var_locglob;
+
+const unique cev_global: var_locglob;
+
+const unique cev_parameter: var_locglob;
+
+const unique cev_implicit: var_locglob;
+
+function #cev_init(n: int) returns (bool);
+
+function #cev_save_position(n: int) returns ($token);
+
+function #cev_var_intro<T,U>(n: int, locorglob: var_locglob, name: $token, val: T, typ: U) returns (bool);
+
+function #cev_var_update<T>(n: int, locorglob: var_locglob, name: $token, val: T) returns (bool);
+
+function #cev_control_flow_event(n: int, tag: cf_event) returns (bool);
+
+function #cev_function_call(n: int) returns (bool);
+
+var #cev_pc: int;
+
+procedure CevVarIntro<T>(pos: $token, locorglob: var_locglob, name: $token, val: T);
+  modifies #cev_pc;
+  ensures #cev_var_intro(old(#cev_pc), locorglob, name, val, 0);
+  ensures #cev_save_position(old(#cev_pc)) == pos;
+  ensures #cev_pc == old(#cev_pc) + 1;
+
+
+
+procedure CevUpdateHere<T>(name: $token, val: T);
+  ensures #cev_var_update(#cev_pc, cev_local, name, val);
+
+
+
+procedure CevStep(pos: $token);
+  modifies #cev_pc;
+  ensures #cev_save_position(old(#cev_pc)) == pos;
+  ensures #cev_pc == old(#cev_pc) + 1;
+
+
+
+procedure CevUpdate<T>(pos: $token, name: $token, val: T);
+  modifies #cev_pc;
+  ensures #cev_var_update(old(#cev_pc), cev_local, name, val);
+  ensures #cev_save_position(old(#cev_pc)) == pos;
+  ensures #cev_pc == old(#cev_pc) + 1;
+
+
+
+procedure CevUpdateHeap(pos: $token, name: $token, val: HeapType);
+  modifies #cev_pc;
+  ensures #cev_var_update(old(#cev_pc), cev_implicit, name, val);
+  ensures #cev_save_position(old(#cev_pc)) == pos;
+  ensures #cev_pc == old(#cev_pc) + 1;
+
+
+
+procedure CevEvent(pos: $token, tag: cf_event);
+  modifies #cev_pc;
+  ensures #cev_control_flow_event(old(#cev_pc), tag);
+  ensures #cev_save_position(old(#cev_pc)) == pos;
+  ensures #cev_pc == old(#cev_pc) + 1;
+
+
+
+procedure CevStepEvent(pos: $token, tag: cf_event);
+  modifies #cev_pc;
+  ensures #cev_control_flow_event(old(#cev_pc) + 1, tag);
+  ensures #cev_save_position(old(#cev_pc) + 1) == pos;
+  ensures #cev_pc == old(#cev_pc) + 2;
+
+
+
+procedure CevPreLoop(pos: $token) returns (oldPC: int);
+  modifies #cev_pc;
+  ensures #cev_control_flow_event(old(#cev_pc), conditional_moment);
+  ensures #cev_save_position(old(#cev_pc)) == pos;
+  ensures oldPC == old(#cev_pc) && #cev_pc == old(#cev_pc) + 1;
+
+
+
+const unique class.C: ClassName;
+
+axiom DeclType(C.w) == class.C;
+
+const unique C.w: Field DatatypeType;
+
+axiom (forall $h: HeapType, $o: ref :: { $h[$o, C.w] } $IsGoodHeap($h) && $o != null && $h[$o, alloc] ==> $h[$o, C.w] == null || ($h[$h[$o, C.w], alloc] && dtype($h[$o, C.w]) == class.WildData));
+
+axiom DeclType(C.list) == class.C;
+
+const unique C.list: Field DatatypeType;
+
+axiom (forall $h: HeapType, $o: ref :: { $h[$o, C.list] } $IsGoodHeap($h) && $o != null && $h[$o, alloc] ==> $h[$o, C.list] == null || ($h[$h[$o, C.list], alloc] && dtype($h[$o, C.list]) == class.List && TypeParams($h[$o, C.list], 0) == class.bool));
